RocqOfRust/revm/revm_interpreter/simulate/instruction_context.v
@@ -1,0 +1,59 @@
+Require Import simulate.RocqOfRust.
+Require Import revm.revm_interpreter.links.instruction_context.
+Require Import revm.revm_interpreter.links.interpreter.
+Require Import revm.revm_interpreter.links.interpreter_types.
+
+Module InstructionContext.
+  Record State
+      (H WIRE : Set) `{Link H} `{Link WIRE}
+      (WIRE_types : InterpreterTypes.Types.t)
+      `{InterpreterTypes.Types.AreLinks WIRE_types} : Set := {
+    state_interpreter : Interpreter.t WIRE WIRE_types;
+    state_host : H;
+  }.
+
+  Definition make
+      {H WIRE : Set} `{Link H} `{Link WIRE}
+      {WIRE_types : InterpreterTypes.Types.t}
+      `{InterpreterTypes.Types.AreLinks WIRE_types} :
+      instruction_context.InstructionContext.t H WIRE WIRE_types :=
+    {|
+      instruction_context.InstructionContext.interpreter := make_ref 0;
+      instruction_context.InstructionContext.host := make_ref 1;
+    |}.
+
+  Definition context
+      {H WIRE : Set} `{Link H} `{Link WIRE}
+      {WIRE_types : InterpreterTypes.Types.t}
+      `{InterpreterTypes.Types.AreLinks WIRE_types}
+      (_state : State H WIRE WIRE_types) :
+      instruction_context.InstructionContext.t H WIRE WIRE_types :=
+    make.
+
+  Definition stack
+      {H WIRE : Set} `{Link H} `{Link WIRE}
+      {WIRE_types : InterpreterTypes.Types.t}
+      `{InterpreterTypes.Types.AreLinks WIRE_types}
+      (state : State H WIRE WIRE_types) : Stack.t :=
+    match state with
+    | {| state_interpreter := interpreter; state_host := host |} =>
+        [interpreter; host]%stack
+    end.
+
+  Definition map_interpreter
+      {H WIRE : Set} `{Link H} `{Link WIRE}
+      {WIRE_types : InterpreterTypes.Types.t}
+      `{InterpreterTypes.Types.AreLinks WIRE_types}
+      (f :
+        Interpreter.t WIRE WIRE_types ->
+        Interpreter.t WIRE WIRE_types)
+      (state : State H WIRE WIRE_types) :
+      State H WIRE WIRE_types :=
+    match state with
+    | {| state_interpreter := interpreter; state_host := host |} =>
+        {|
+          state_interpreter := f interpreter;
+          state_host := host;
+        |}
+    end.
+End InstructionContext.
